ver3_less_complex/Adversary.dfy
@@ -21,7 +21,7 @@ module M_Adversary {
     predicate AdversaryInit(a : Adversary)
     {
         && a.byz_nodes == M_SpecTypes.Adversary_Nodes
-        &&  a.byz_nodes <= M_SpecTypes.All_Nodes  // byzantine nodes should exists in the set of all nodes.
+        && a.byz_nodes <= M_SpecTypes.All_Nodes  // byzantine nodes should exists in the set of all nodes.
         && |a.byz_nodes| <= f(|M_SpecTypes.All_Nodes|)    // the counts of byzantine nodes should not exceed 1/3 of all nodes.
     }
 
